theories/ExprProp.v
@@ -1,5 +1,4 @@
 Require Import ExtLib.Structures.Traversable.
-Require Import ExtLib.Data.List.
 Require Import ExtLib.Data.HList.
 Require Import ExtLib.Tactics.
 Require Import MirrorCore.ExprI.
