theories/ExprSem.v
@@ -1,8 +1,5 @@
-Require Import Coq.Classes.Morphisms.
 Require Import Coq.Relations.Relations.
-Require Import MirrorCore.EnvI.
 Require Import MirrorCore.ExprI.
-Require Import MirrorCore.TypesI.
 
 Set Implicit Arguments.
 Set Strict Implicit.
