theories/Lambda/RewriteRelations.v
@@ -1,0 +1,545 @@
+Require Import ExtLib.Core.RelDec.
+Require Import ExtLib.Data.HList.
+Require Import ExtLib.Tactics.
+Require Import MirrorCore.Lemma.
+Require Import MirrorCore.Util.Forwardy.
+Require Import MirrorCore.Util.Compat.
+Require Import MirrorCore.ExprI.
+Require Import MirrorCore.Lambda.Expr.
+Require Import MirrorCore.Lambda.ExprTac.
+Require Import MirrorCore.Views.Ptrns.
+
+Set Implicit Arguments.
+Set Strict Implicit.
+
+Section setoid.
+  Context {typ : Type}.
+  Context {func : Type}.
+  Context {RType_typD : RType typ}.
+  Context {Typ2_Fun : Typ2 RType_typD Fun}.
+  Context {RSym_func : RSym func}.
+
+  (** Reasoning principles **)
+  Context {RTypeOk_typD : RTypeOk}.
+  Context {Typ2Ok_Fun : Typ2Ok Typ2_Fun}.
+  Context {RSymOk_func : RSymOk RSym_func}.
+  Context {Typ0_Prop : Typ0 _ Prop}.
+  Context {RelDec_eq_typ : RelDec (@eq typ)}.
+  Context {RelDec_Correct_eq_typ : RelDec_Correct RelDec_eq_typ}.
+
+  Let tyArr : typ -> typ -> typ := @typ2 _ _ _ _.
+
+  Variable Rbase : Type.
+  Variable Rbase_eq : Rbase -> Rbase -> bool.
+  Hypothesis Rbase_eq_ok : forall a b, Rbase_eq a b = true -> a = b.
+
+  Inductive R : Type :=
+  | Rinj (r : Rbase)
+  | Rrespects (l r : R)
+  | Rpointwise (t : typ) (r : R)
+  | Rflip (r : R).
+
+  Definition Rflip' (r : R) : R :=
+    match r with
+    | Rflip r => r
+    | _ => Rflip r
+    end.
+
+  Fixpoint Req_dec (a b : R) : bool :=
+    match a , b with
+    | Rinj a , Rinj b => Rbase_eq a b
+    | Rrespects l r , Rrespects l' r' =>
+      if Req_dec l l' then Req_dec r r' else false
+    | Rpointwise t a , Rpointwise t' a' =>
+      if t ?[ eq ] t' then Req_dec a a' else false
+    | Rflip a , Rflip b => Req_dec a b
+    | _ , _ => false
+    end.
+
+  Theorem Req_dec_ok : forall x y : R, Req_dec x y = true -> x = y.
+  Proof.
+    clear - RTypeOk_typD Rbase_eq_ok RelDec_Correct_eq_typ.
+    induction x; destruct y; simpl; try solve [ congruence ].
+    { intros.
+      eapply Rbase_eq_ok in H. destruct H; reflexivity. }
+    { specialize (IHx1 y1).
+      specialize (IHx2 y2).
+      destruct (Req_dec x1 y1); intros; try congruence.
+      destruct (Req_dec x2 y2); intros; try congruence.
+      f_equal; tauto. }
+    { consider (t ?[ eq ] t0); intros.
+      { subst. f_equal; eauto. } }
+    { intros. eapply IHx in H. f_equal. assumption. }
+  Qed.
+
+  Variable RbaseD : Rbase -> forall t : typ, option (typD t -> typD t -> Prop).
+
+  Hypothesis RbaseD_single_type
+  : forall r t1 t2 rD1 rD2,
+      RbaseD r t1 = Some rD1 ->
+      RbaseD r t2 = Some rD2 ->
+      t1 = t2.
+
+  (** This is due to universe problems! **)
+  Definition respectful :=
+    fun (A B : Type) (R : A -> A -> Prop) (R' : B -> B -> Prop)
+        (f g : A -> B) =>
+      forall x y : A, R x y -> R' (f x) (g y).
+
+  Definition pointwise_relation :=
+    fun (A B : Type) (R : B -> B -> Prop) (f g : A -> B) =>
+      forall a : A, R (f a) (g a).
+
+  Definition flip (A : Type) (R : A -> A -> Prop) : A -> A -> Prop :=
+    fun x y => R y x.
+
+  Fixpoint RD (r : R) (t : typ) : option (typD t -> typD t -> Prop) :=
+    match r with
+      | Rinj r => RbaseD r t
+      | Rrespects l r =>
+        typ2_match (F:=Fun) (fun T => option (T -> T -> Prop)) t
+                   (fun lt rt =>
+                      match RD l lt , RD r rt with
+                        | Some l , Some r => Some (respectful l r)
+                        | _ , _ => None
+                      end)
+                   None
+      | Rpointwise _t r =>
+        typ2_match (F:=Fun) (fun T => option (T -> T -> Prop)) t
+                   (fun lt rt =>
+                      match type_cast t _t with
+                        | Some _ =>
+                          match RD r rt with
+                            | Some r => Some (pointwise_relation (A:=typD lt) r)
+                            | _ => None
+                          end
+                        | None => None
+                      end)
+                   None
+      | Rflip r =>
+        match RD r t with
+        | Some rD => Some (flip rD)
+        | None => None
+        end
+    end.
+
+  Theorem RD_single_type
+  : forall r t1 t2 rD1 rD2,
+      RD r t1 = Some rD1 ->
+      RD r t2 = Some rD2 ->
+      t1 = t2.
+  Proof using tyArr RbaseD_single_type Typ2Ok_Fun.
+    induction r; simpl; intros.
+    { eapply RbaseD_single_type; eauto. }
+    { destruct (typ2_match_case t2) as [ [ ? [ ? [ ? H1 ] ] ] | H1 ];
+        rewrite H1 in *; [ clear H1 | congruence ].
+      destruct (typ2_match_case t1) as [ [ ? [ ? [ ? H1 ] ] ] | H1 ];
+        rewrite H1 in *; [ clear H1 | congruence ].
+      revert H; revert H0.
+      red in x4; red in x1; subst.
+      simpl.
+      autorewrite_with_eq_rw.
+      intros; forwardy; inv_all; subst.
+      f_equal; eauto. }
+    { destruct (typ2_match_case t2) as [ [ ? [ ? [ ? H1 ] ] ] | H1 ];
+        rewrite H1 in *; [ clear H1 | congruence ].
+      destruct (typ2_match_case t1) as [ [ ? [ ? [ ? H1 ] ] ] | H1 ];
+        rewrite H1 in *; [ clear H1 | congruence ].
+      revert H; revert H0.
+      red in x4; red in x1; subst.
+      simpl.
+      autorewrite_with_eq_rw.
+      intros; forwardy; inv_all; subst.
+      red in y0, y3; subst.
+      f_equal; eauto.
+      clear H0; eapply typ2_inj in y3; eauto.
+      symmetry. tauto. }
+    { forwardy.
+      inv_all. subst. eauto. }
+  Qed.
+
+  Ltac ptrn_contradict :=
+    match goal with
+    | H : forall (x : _), forall y, forall z, z _ = y _ |- _ =>
+      exfalso; clear - H;
+      specialize (H _ (fun _ => true) (fun _ => false)); simpl in H; congruence
+    | H : forall (x : _), forall y, forall z, y _ = z _ |- _ =>
+      exfalso; clear - H;
+      specialize (H _ (fun _ => true) (fun _ => false)); simpl in H; congruence
+    end.
+
+  (** Patterns *)
+  Definition ptrnRinj {T : Type} (p : ptrn Rbase T) : ptrn R T :=
+    fun r _T good bad =>
+      match r with
+      | Rinj a => p a _T good (fun x => bad (Rinj x))
+      | Rrespects a b => bad (Rrespects a b)
+      | Rpointwise a b => bad (Rpointwise a b)
+      | Rflip a => bad (Rflip a)
+      end.
+
+  Global Instance ptrn_ok_ptrnRinj {T} p : ptrn_ok p -> ptrn_ok (@ptrnRinj T p).
+  Proof using.
+    unfold ptrnRinj; red; intros.
+    destruct x; simpl; try solve [ right; red; eauto ].
+    destruct (H r).
+    { left; destruct H0. exists x. red. eauto. }
+    { right. red. red in H0. intros.
+      setoid_rewrite H0. reflexivity. }
+  Qed.
+
+  Theorem Succeeds_ptrnRinj {T} p x res
+  : ptrn_ok p ->
+    Succeeds x (@ptrnRinj T p) res ->
+    exists y, Succeeds y p res /\ x = Rinj y.
+  Proof using.
+    destruct x; unfold Succeeds; simpl; intros;
+    try solve [ ptrn_contradict ].
+    eexists; split; eauto.
+    intros.
+    destruct (H r) as [ [ ? ? ] | ? ].
+    { red in H1. setoid_rewrite H1 in H0. setoid_rewrite H1. eauto. }
+    { red in H1. setoid_rewrite H1 in H0.
+      ptrn_contradict. }
+  Qed.
+
+  Global Instance SucceedsE_ptrnRinj {T} p x res
+  : ptrn_ok p -> SucceedsE x (@ptrnRinj T p) res :=
+  { s_result := exists y, Succeeds y p res /\ x = Rinj y }.
+  intros.  eauto using Succeeds_ptrnRinj.
+  Defined.
+
+  Definition ptrnRflip {T : Type} (p : ptrn R T)
+  : ptrn R T :=
+    fun r _T good bad =>
+      match r with
+      | Rinj a => bad (Rinj a)
+      | Rrespects a b => bad (Rrespects a b)
+      | Rpointwise a b => bad (Rpointwise a b)
+      | Rflip a => p a _T good (fun x => bad (Rflip x))
+      end.
+
+  Global Instance ptrn_ok_ptrnRflip {T} p : ptrn_ok p -> ptrn_ok (@ptrnRflip T p).
+  Proof using.
+    unfold ptrnRflip; red; intros.
+    destruct x; simpl; try solve [ right; red; eauto ].
+    destruct (H x).
+    { left; destruct H0. exists x0. red. eauto. }
+    { right. red. red in H0. intros.
+      setoid_rewrite H0. reflexivity. }
+  Qed.
+
+  Theorem Succeeds_ptrnRflip {T} p x res
+  : ptrn_ok p ->
+    Succeeds x (@ptrnRflip T p) res ->
+    exists y, Succeeds y p res /\ x = Rflip y.
+  Proof using.
+    destruct x; unfold Succeeds; simpl; intros;
+    try solve [ ptrn_contradict ].
+    eexists; split; eauto.
+    intros.
+    destruct (H x) as [ [ ? ? ] | ? ].
+    { red in H1. setoid_rewrite H1 in H0. setoid_rewrite H1. eauto. }
+    { red in H1. setoid_rewrite H1 in H0.
+      ptrn_contradict. }
+  Qed.
+
+  Global Instance SucceedsE_ptrnRflip {T} p x res
+  : ptrn_ok p -> SucceedsE x (@ptrnRflip T p) res :=
+  { s_result := exists y, Succeeds y p res /\ x = Rflip y }.
+  intros.  eauto using Succeeds_ptrnRflip.
+  Defined.
+
+  Definition ptrnRrespectsL {T U : Type}
+             (pd : ptrn R (T -> U))
+             (pr : ptrn R T)
+  : ptrn R U :=
+    fun r _T good bad =>
+      match r with
+      | Rinj a => bad (Rinj a)
+      | Rrespects a b => pr b _T (fun x => pd a _T (fun y => good (y x))
+                                              (fun a => bad (Rrespects a b)))
+                            (fun b => bad (Rrespects a b))
+      | Rpointwise a b => bad (Rpointwise a b)
+      | Rflip a => bad (Rflip a)
+      end.
+
+  Global Instance ptrn_ok_ptrnRrespectsL {T U} pl pr
+  : ptrn_ok pl -> ptrn_ok pr -> ptrn_ok (@ptrnRrespectsL T U pl pr).
+  Proof using.
+    unfold ptrnRrespectsL; red; intros.
+    destruct x; simpl; try solve [ right; red; eauto ].
+    destruct (H x1); destruct (H0 x2).
+    { forward_reason. left.
+      unfold Succeeds in *. exists (x0 x). intros.
+      setoid_rewrite H2. setoid_rewrite H1. reflexivity. }
+    { right. red. red in H2.
+      setoid_rewrite H2. eauto. }
+    { right. destruct H2. red in H1, H2.
+      red. setoid_rewrite H2. setoid_rewrite H1. eauto. }
+    { right. red in H1, H2.
+      red. setoid_rewrite H2. eauto. }
+  Qed.
+
+  Theorem Succeeds_ptrnRrespectsL {T U} pl pr x res
+  : ptrn_ok pl -> ptrn_ok pr ->
+    Succeeds x (@ptrnRrespectsL T U pl pr) res ->
+    exists y z resL resR, Succeeds y pl resL /\ Succeeds z pr resR /\
+                          x = Rrespects y z /\ res = resL resR.
+  Proof using.
+    destruct x; unfold Succeeds; simpl; intros;
+    try solve [ ptrn_contradict ].
+    exists x1; exists x2.
+    destruct (H0 x2).
+    { destruct H2; red in H2. setoid_rewrite H2 in H1.
+      destruct (H x1).
+      { destruct H3; red in H3; setoid_rewrite H3 in H1.
+        do 2 eexists. split; eauto. split; eauto.
+        split; eauto.
+        specialize (H1 _ (fun x => x) (fun _ => res)).
+        symmetry; assumption. }
+      { red in H3. setoid_rewrite H3 in H1.
+        ptrn_contradict. } }
+    { red in H2. setoid_rewrite H2 in H1. ptrn_contradict. }
+  Qed.
+
+  Global Instance SucceedsE_ptrnRrespectsL {T U} pl pr x res
+  : ptrn_ok pl -> ptrn_ok pr -> SucceedsE x (@ptrnRrespectsL T U pl pr) res :=
+  { s_result := exists y z resL resR, Succeeds y pl resL /\ Succeeds z pr resR /\
+                          x = Rrespects y z /\ res = resL resR }.
+  intros.  eauto using Succeeds_ptrnRrespectsL.
+  Defined.
+
+  Definition ptrnRpointwiseL {T U : Type}
+             (pd : ptrn typ (T -> U))
+             (pr : ptrn R T)
+  : ptrn R U :=
+    fun r _T good bad =>
+      match r with
+      | Rinj a => bad (Rinj a)
+      | Rpointwise a b => pr b _T (fun x => pd a _T (fun y => good (y x))
+                                              (fun a => bad (Rpointwise a b)))
+                            (fun b => bad (Rpointwise a b))
+      | Rrespects a b => bad (Rrespects a b)
+      | Rflip a => bad (Rflip a)
+      end.
+
+  Global Instance ptrn_ok_ptrnRpointwiseL {T U} pl pr
+  : ptrn_ok pl -> ptrn_ok pr -> ptrn_ok (@ptrnRpointwiseL T U pl pr).
+  Proof using.
+    unfold ptrnRpointwiseL; red; intros.
+    destruct x; simpl; try solve [ right; red; eauto ].
+    destruct (H t); destruct (H0 x).
+    { forward_reason. left.
+      unfold Succeeds in *. setoid_rewrite H2.
+      setoid_rewrite H1. eauto. }
+    { right. red. red in H2.
+      setoid_rewrite H2. eauto. }
+    { right. destruct H2. red in H1, H2.
+      red. setoid_rewrite H2. setoid_rewrite H1. eauto. }
+    { right. red in H1, H2.
+      red. setoid_rewrite H2. eauto. }
+  Qed.
+
+  Theorem Succeeds_ptrnRpointwiseL {T U} pl pr x res
+  : ptrn_ok pl -> ptrn_ok pr ->
+    Succeeds x (@ptrnRpointwiseL T U pl pr) res ->
+    exists y z resL resR, Succeeds y pl resL /\ Succeeds z pr resR /\
+                          x = Rpointwise y z /\ res = resL resR.
+  Proof using.
+    destruct x; unfold Succeeds; simpl; intros;
+    try solve [ ptrn_contradict ].
+    exists t; exists x.
+    destruct (H0 x).
+    { destruct H2; red in H2. setoid_rewrite H2 in H1.
+      destruct (H t).
+      { destruct H3; red in H3; setoid_rewrite H3 in H1.
+        do 2 eexists. split; eauto. split; eauto.
+        split; eauto.
+        specialize (H1 _ (fun x => x) (fun _ => res)).
+        symmetry; assumption. }
+      { red in H3. setoid_rewrite H3 in H1.
+        ptrn_contradict. } }
+    { red in H2. setoid_rewrite H2 in H1. ptrn_contradict. }
+  Qed.
+
+  Global Instance SucceedsE_ptrnRpointwiseL {T U} pl pr x res
+  : ptrn_ok pl -> ptrn_ok pr -> SucceedsE x (@ptrnRpointwiseL T U pl pr) res :=
+  { s_result := exists y z resL resR, Succeeds y pl resL /\ Succeeds z pr resR /\
+                          x = Rpointwise y z /\ res = resL resR }.
+  intros.  eauto using Succeeds_ptrnRpointwiseL.
+  Defined.
+
+  (** Reflexivity and transitivity *)
+  Section is_trans_refl.
+
+    Lemma Refl_pointwise : forall {T U : Type} (R : T -> T -> Prop),
+      Reflexive R -> Reflexive (pointwise_relation (A:=U) R).
+    Proof using.
+      compute. auto.
+    Qed.
+
+    Lemma Trans_pointwise : forall {T U : Type} (R : T -> T -> Prop),
+        Transitive R -> Transitive (pointwise_relation (A:=U) R).
+    Proof using.
+      compute. eauto.
+    Qed.
+
+    Variable is_trans : Rbase -> bool.
+    Fixpoint is_transR (r : R) : bool :=
+      match r with
+      | Rinj r => is_trans r
+      | Rpointwise _ x => is_transR x
+      | Rflip r => is_transR r
+      | _ => false
+      end.
+
+    Definition is_reflR := is_transR.
+
+    Hypothesis is_transOk : forall r t rD,
+        is_trans r = true -> RbaseD r t = Some rD -> Transitive rD.
+
+    Theorem is_transROk : forall r t rD,
+        is_transR r = true -> RD r t = Some rD -> Transitive rD.
+    Proof using Typ2Ok_Fun is_transOk.
+      induction r; simpl; intros; eauto; try congruence.
+      { simpl. intros.
+        destruct (typ2_match_case t0) as [ [ ? [ ? [ ? H1 ] ] ] | H1 ];
+          rewrite H1 in *; [ clear H1 | congruence ].
+        revert H0.
+        red in x1; subst; simpl.
+        autorewrite_with_eq_rw.
+        intros. forwardy; inv_all; subst.
+        eapply IHr in H; [ | eassumption ].
+        red.
+        do 3 intro. autorewrite_with_eq_rw.
+        eapply Trans_pointwise. eassumption. }
+      { forwardy; inv_all; subst.
+        red. intros. unfold flip. eapply IHr; eauto. }
+    Qed.
+
+    Hypothesis is_reflOk : forall r t rD,
+        is_trans r = true -> RbaseD r t = Some rD -> Reflexive rD.
+
+    Theorem is_reflROk : forall r t rD,
+        is_reflR r = true -> RD r t = Some rD -> Reflexive rD.
+    Proof using Typ2Ok_Fun is_reflOk.
+      induction r; simpl; intros; eauto; try congruence.
+      { simpl. intros.
+        destruct (typ2_match_case t0) as [ [ ? [ ? [ ? H1 ] ] ] | H1 ];
+          rewrite H1 in *; [ clear H1 | congruence ].
+        revert H0.
+        red in x1; subst; simpl.
+        autorewrite_with_eq_rw.
+        intros. forwardy; inv_all; subst.
+        eapply IHr in H; [ | eassumption ].
+        red.
+        intro. autorewrite_with_eq_rw.
+        eapply Refl_pointwise. eassumption. }
+      { forwardy; inv_all; subst.
+        red. intros. unfold flip. eapply IHr; eauto. }
+    Qed.
+
+  End is_trans_refl.
+
+  (** Rewriting Lemmas **)
+  Section lemmas.
+    (** Note: This could be parameterized by the type of expressions
+     **)
+    Existing Instance Expr_expr.
+
+    Record rw_concl : Type :=
+    { lhs : expr typ func
+    ; rel : R
+    ; rhs : expr typ func }.
+
+    Definition rw_lemma : Type :=
+      Lemma.lemma typ (expr typ func) rw_concl.
+
+    Definition rw_conclD (tus tvs : tenv typ) (c : rw_concl)
+    : option (exprT tus tvs Prop) :=
+      match typeof_expr tus tvs c.(lhs) with
+      | None => None
+      | Some t =>
+        match exprD' tus tvs t c.(lhs)
+            , exprD' tus tvs t c.(rhs)
+            , RD c.(rel) t
+        with
+        | Some lhs , Some rhs , Some rel =>
+          Some (fun us vs => rel (lhs us vs) (rhs us vs))
+        | _ , _ , _ => None
+        end
+      end.
+
+    Lemma rw_concl_weaken
+    : forall (tus tvs : tenv typ) (l : rw_concl) (lD : exprT tus tvs Prop),
+        rw_conclD tus tvs l = Some lD ->
+        forall tus' tvs' : list typ,
+        exists lD' : exprT (tus ++ tus') (tvs ++ tvs') Prop,
+          rw_conclD (tus ++ tus') (tvs ++ tvs') l = Some lD' /\
+          (forall (us : hlist typD tus) (us' : hlist typD tus')
+                  (vs : hlist typD tvs) (vs' : hlist typD tvs'),
+              lD us vs <-> lD' (hlist_app us us') (hlist_app vs vs')).
+    Proof.
+      unfold rw_conclD. simpl. intros.
+      forwardy. inv_all. subst.
+      erewrite ExprFacts.typeof_expr_weaken by eauto.
+      eapply ExprFacts.exprD'_weaken in H0; eauto.
+      destruct H0 as [ ? [ Hx ? ] ]; rewrite Hx; clear Hx.
+      eapply ExprFacts.exprD'_weaken in H1; eauto.
+      destruct H1 as [ ? [ Hx ? ] ]; rewrite Hx; clear Hx.
+      rewrite H2. eexists; split; eauto.
+      intros. simpl. rewrite <- H0. rewrite <- H1. reflexivity.
+    Qed.
+
+
+    Definition flip_rw_concl (a : rw_concl) : rw_concl :=
+    {| lhs := a.(rhs)
+     ; rel := Rflip' a.(rel)
+     ; rhs := a.(lhs)
+     |}.
+
+    Definition flip_rw_lemma (lem : rw_lemma) : rw_lemma :=
+    {| vars := lem.(vars)
+     ; premises := lem.(premises)
+     ; concl := flip_rw_concl lem.(concl) |}.
+
+    Lemma RD_Rflip'_Rflip : forall a b,
+        RD (Rflip' a) b = RD (Rflip a) b.
+    Proof.
+      destruct a; simpl; eauto.
+      intros. destruct (RD a b); reflexivity.
+    Qed.
+
+    Theorem flip_rw_lemma_sound
+    : forall (lem : rw_lemma),
+        lemmaD rw_conclD nil nil lem ->
+        lemmaD rw_conclD nil nil (flip_rw_lemma lem).
+    Proof using RTypeOk_typD Typ2Ok_Fun RSymOk_func.
+      unfold lemmaD, lemmaD'. simpl.
+      intros. forwardy.
+      Cases.rewrite_all_goal.
+      destruct (concl lem); simpl in *.
+      unfold flip_rw_concl. simpl.
+      unfold rw_conclD in *. simpl in *.
+      forwardy.
+      erewrite exprD_typeof_Some; eauto.
+      Cases.rewrite_all_goal.
+      rewrite RD_Rflip'_Rflip.
+      simpl.
+      Cases.rewrite_all_goal.
+      inv_all.
+      subst. unfold flip. eauto.
+    Qed.
+
+  End lemmas.
+
+End setoid.
+
+Arguments rw_concl typ func Rbase : rename, clear implicits.
+Arguments rw_lemma typ func Rbase : rename, clear implicits.
+Arguments R typ Rbase : rename, clear implicits.
+Arguments Rrespects {_ _} _ _.
+Arguments Rpointwise {_ _} _ _.
+Arguments Rflip {_ _} _.
+Arguments Rinj {_ _} _.
