theories/Lemma.v
@@ -1,4 +1,3 @@
-Require Import ExtLib.Data.List.
 Require Import ExtLib.Data.HList.
 Require Import ExtLib.Tactics.
 Require Import MirrorCore.Util.Compat.
