theories/VariablesI.v
@@ -1,13 +1,6 @@
-Require Import Coq.Bool.Bool.
-Require Import Coq.Lists.List.
-Require Import Coq.Classes.Morphisms.
-Require Import ExtLib.Core.RelDec.
 Require Import ExtLib.Data.HList.
-Require Import ExtLib.Data.Eq.
 Require Import ExtLib.Tactics.
-Require Import MirrorCore.TypesI.
 Require Import MirrorCore.ExprI.
-Require Import MirrorCore.EnvI.
 Require Import MirrorCore.CtxLogic.
 
 Set Implicit Arguments.
