theories/syms/SymSum.v
@@ -1,7 +1,3 @@
-Require Import ExtLib.Core.RelDec.
-Require Import ExtLib.Data.Map.FMapPositive.
-Require Import ExtLib.Data.SumN.
-
 Require Import MirrorCore.SymI.
 Require Import MirrorCore.TypesI.
 
